Source/DafnyStandardLibraries/src/Std/JSON/ByteStrConversion.dfy
@@ -6,7 +6,7 @@
 /**
  Derives conversions to and from sequences of bytes.
  */
-module Std.JSON.ByteStrConversion refines Strings.ParametricConversion {
+module {:disableNonlinearArithmetic} Std.JSON.ByteStrConversion refines Strings.ParametricConversion {
   import opened BoundedInts
 
   type Char = byte
